fstar/Spec.Signal.Core.fst
@@ -7,7 +7,9 @@ open Lib.RawIntTypes
 open Spec.Signal.Crypto
 open Spec.Signal.Messages
 
-#set-options "--max_fuel 0 --initial_fuel 0 --initial_ifuel 0 --max_ifuel 0 --z3rlimit 50"
+
+#set-options "--z3rlimit 50 --fuel 0 --ifuel 0"
+
 
 let verify_sig (identity_key:pubkey) (signed_pub_key: pubkey) (signature:lbytes 64) : Tot bool =
   verify identity_key signed_pub_key signature
@@ -15,14 +17,15 @@ let verify_sig (identity_key:pubkey) (signed_pub_key: pubkey) (signature:lbytes 
 let sign (priv_key:privkey) (pub_key:pubkey) : Tot (lbytes 64) =
   sign priv_key pub_key
 
+
 let ratchet
     (root_key:key)                   (* $rk_j$    *)
     (our_ephemeral_priv_key:privkey) (* $x_j$     *)
     (their_ephemeral_pub_key:pubkey) (* $g^{y_j}$ *)
-    : Tot (key & key) =                  (* output: $rk_{j+1}, ck_{j+1,0}$ *)
+    : Tot (key & key) =              (* output: $rk_{j+1}, ck_{j+1,0}$ *)
 
-  let shared_secret = dh our_ephemeral_priv_key
-			 their_ephemeral_pub_key in
+  let shared_secret =
+    dh our_ephemeral_priv_key their_ephemeral_pub_key in
   let keys = hkdf2 shared_secret root_key label_WhisperRatchet in
   let root_key' = sub keys 0 32 in
   let chain_key = sub keys 32 32 in
@@ -44,11 +47,11 @@ let initiate'
     match their_onetime_pub_key with
     | None -> ff @| dh1 @| dh2 @| dh3
     | Some their_onetime_pub_key ->
-	let dh4 = dh our_onetime_priv_key their_onetime_pub_key in
-	ff @| dh1 @| dh2 @| dh3 @| dh4
-  in
+	   let dh4 = dh our_onetime_priv_key their_onetime_pub_key in
+	   ff @| dh1 @| dh2 @| dh3 @| dh4 in
   let res = hkdf1 shared_secret zz label_WhisperText in
   res
+
 
 let initiate
     (our_identity_priv_key: privkey) (* $i$   *)
@@ -95,6 +98,7 @@ let fill_message_keys
   let chain_key' = hmac chain_key two in
   msg_key, chain_key'
 
+
 let size_encrypt_max_length
   (plen:size_nat{plen + 16 <= max_size_t /\ cipherlen plen + 140 <= max_size_t})
   : size_nat =
@@ -107,7 +111,6 @@ let encrypt_get_length
     : Tot (r:size_nat{r <= size_encrypt_max_length plen}) =
     1 + (serialize_whisper_message_get_length prev_counter counter (cipherlen plen)) + 8
 
-#set-options "--z3rlimit 200"
 
 let encrypt
     (our_identity_pub_key:pubkey)    (* $g^i$ or $g^r$ *)
@@ -127,8 +130,11 @@ let encrypt
   (* FStarEncrypt returns here with (ciphertext & mac_key) *)
   let whisper_msg = serialize_whisper_message our_ephemeral_pub_key
 		      prev_counter counter ciphertext in
+  (* BB: 2019/11/04 *)
+  assume(length whisper_msg + size_mac_whisper_msg_extra_info +
+    Spec.Hash.Definitions.block_length (Spec.Hash.Definitions.SHA2_256) < max_size_t);
   let tag8 : lbytes 8 = mac_whisper_msg mac_key their_identity_pub_key our_identity_pub_key whisper_msg in
-  let c0 : lbytes 1 = create 1 (((u8 3) <<. 4ul) |. (u8 3)) in
+  let c0 : lbytes 1 = create 1 (((u8 3) <<. (size 4)) |. (u8 3)) in
   let output = concat (concat c0 (to_lseq whisper_msg)) tag8 in
   output
 
@@ -154,8 +160,7 @@ let decrypt
     serialize_whisper_message remote_ephemeral_key prev_counter counter ciphertext
   in
   let exp_tag8 =
-      mac_whisper_msg mac_key our_identity_pub_key
-			      their_identity_pub_key whisper_message in
+    mac_whisper_msg mac_key our_identity_pub_key their_identity_pub_key whisper_message in
   if not (equal_bytes tag8 exp_tag8) then
     None
   else
@@ -163,6 +168,7 @@ let decrypt
     match plain with
     | Some plain -> Some plain
     | None -> None
+
 
 let generate_key_pair (e: Ghost.erased entropy) : Tot (privkey & pubkey) =
   let priv = random_bytes e 32 in
