fstar/Spec.Signal.Crypto.fst
@@ -5,18 +5,31 @@ open Lib.IntTypes
 open Lib.ByteSequence
 open Lib.Sequence
 
-#reset-options "--initial_fuel 0 --max_fuel 0 --initial_ifuel 0 --max_ifuel 0"
 
-(* BB. Relocate to Spec.Signal.Constants ? *)
+#reset-options "--z3rlimit 50 --fuel 0 --ifuel 0"
+
+let pow2_61 : l:unit{pow2 61 == 2305843009213693952} = assert_norm(pow2 61 == 2305843009213693952)
+
+
+(* Constants *)
 inline_for_extraction let size_privkey = 32
 inline_for_extraction let size_pubkey = 33
 inline_for_extraction let size_key = 32
 inline_for_extraction let size_iv = 16
 inline_for_extraction let size_tag = 32
 inline_for_extraction let size_sigval = 64
-let cipherlen (plen:size_nat{plen + 16 <= max_size_t}) : size_nat =
-  ((plen + 16) / 16) `op_Multiply` 16
 
+inline_for_extraction let five1_list: l:list uint8{List.Tot.length l == 1} =
+  [@ inline_let]
+  let l = [(u8 0x05)] in
+  assert_norm(List.Tot.length l ==1);
+  l
+
+inline_for_extraction noextract
+let five1 : lseq uint8 1 = createL five1_list
+
+
+(* Base Types *)
 type privkey = lbytes size_privkey
 type pubkey = lbytes size_pubkey
 type key = lbytes size_key
@@ -24,19 +37,12 @@ type iv = lbytes size_iv
 type tag = lbytes size_tag
 type sigval = lbytes size_sigval
 
-(* BB. Relocate to Spec.Signal.Constants ? *)
-let pow2_61 : l:unit{pow2 61 == 2305843009213693952} = assert_norm(pow2 61 == 2305843009213693952)
-
-(* BB. Relocate to Spec.Signal.Constants ? *)
-
 let lbytes_sub (x:size_nat) = b:bytes{length b <= x}
 
-inline_for_extraction let five1_list: l:list uint8{List.Tot.length l == 1} =
-  [@ inline_let]
-  let l = [(u8 0x05)] in
-  assert_norm(List.Tot.length l ==1);
-  l
-inline_for_extraction noextract let five1 : lseq uint8 1 = createL five1_list
+(* Compute ciphertext length from plaintex length *)
+let cipherlen (plen:size_nat{plen + 16 <= max_size_t}) : size_nat =
+  ((plen + 16) / 16) `op_Multiply` 16
+
 
 
 val priv_to_pub: our_priv_key:privkey -> our_pub_key:pubkey
@@ -53,28 +59,40 @@ let dh kpriv kpub =
   Spec.Curve25519.scalarmult kpriv raw_kpub
 
 
+val hmac:
+    key:key
+    -> input: bytes{length input +
+      Spec.Hash.Definitions.block_length Spec.Hash.Definitions.SHA2_256 < max_size_t} ->
+  Tot (lbytes 32)
+let hmac mk plain =
+  assert_norm(max_size_t <= pow2 61 - 1 - size_key - 64);
+  Spec.Agile.HMAC.hmac Spec.Hash.Definitions.SHA2_256 mk plain
+
+
 val hkdf1: key:lbytes_sub 160 -> salt:lbytes 32 -> info:lbytes_sub 32  -> Tot (lbytes 32)
 let hkdf1 key salt info =
-  let extracted = Spec.HKDF.hkdf_extract Spec.Hash.Definitions.SHA2_256 salt key in
-  Spec.HKDF.hkdf_expand Spec.Hash.Definitions.SHA2_256 extracted info 32
+  let extracted = Spec.Agile.HKDF.extract Spec.Hash.Definitions.SHA2_256 salt key in
+  Spec.Agile.HKDF.expand Spec.Hash.Definitions.SHA2_256 extracted info 32
 
 val hkdf2: key:lbytes 32 -> salt:lbytes 32 -> info:lbytes_sub 32 -> lbytes 64
 let hkdf2 key salt info =
-  let extracted = Spec.HKDF.hkdf_extract Spec.Hash.Definitions.SHA2_256 salt key in
-  Spec.HKDF.hkdf_expand Spec.Hash.Definitions.SHA2_256 extracted info 64
+  let extracted = Spec.Agile.HKDF.extract Spec.Hash.Definitions.SHA2_256 salt key in
+  Spec.Agile.HKDF.expand Spec.Hash.Definitions.SHA2_256 extracted info 64
 
 val hkdf3: key:lbytes 32 -> salt:lbytes 32 -> info:lbytes_sub 32 -> lbytes 96
 let hkdf3 key salt info =
-  let extracted = Spec.HKDF.hkdf_extract Spec.Hash.Definitions.SHA2_256 salt key in
-  Spec.HKDF.hkdf_expand Spec.Hash.Definitions.SHA2_256 extracted info 96
+  let extracted = Spec.Agile.HKDF.extract Spec.Hash.Definitions.SHA2_256 salt key in
+  Spec.Agile.HKDF.expand Spec.Hash.Definitions.SHA2_256 extracted info 96
+
 
 val aes_enc:
   ek:key ->
   iv:iv ->
   plain:bytes{length plain + Spec.AES256.blocklen <= max_size_t}  ->
   Tot (cipher:bytes{length cipher <= length plain + 16})
+
 let aes_enc ek iv plain =
-   Spec.AES256_CBC.aes256_cbc_encrypt ek iv plain (length plain)
+  Spec.AES256_CBC.aes256_cbc_encrypt ek iv plain (length plain)
 
 
 val aes_dec:
@@ -91,20 +109,11 @@ val aes_dec:
 let aes_dec ek iv cipher =
   Spec.AES256_CBC.aes256_cbc_decrypt ek iv cipher (length cipher)
 
-val hmac:
-    key:key
-    -> input: bytes{length input +
-      Spec.Hash.Definitions.block_length Spec.Hash.Definitions.SHA2_256 < max_size_t} ->
-  Tot (lbytes 32)
-let hmac mk plain =
-  assert_norm(max_size_t <= pow2 61 - 1 - size_key - 64);
-  Spec.HMAC.hmac Spec.Hash.Definitions.SHA2_256 mk plain
-
 
 val sign: sk:privkey -> plain:bytes{8 * length plain < max_size_t} -> sv:sigval
 let sign sk plain =
   let len = length plain in
-  let ed_key = concat #uint8 #32 #32 sk 
+  let ed_key = concat #uint8 #32 #32 sk
     (Spec.Ed25519.point_compress (Spec.Ed25519.point_mul sk Spec.Ed25519.g)) in
   let sign_bit = index ed_key 63 &. u8 0x80 in
   let sk = sub ed_key 0 32 in
@@ -116,6 +125,7 @@ let sign sk plain =
   let s = (r + (h * nat_from_bytes_le sk) % Spec.Ed25519.q) % Spec.Ed25519.q in
   let sig = concat #uint8 #32 #32 rs (nat_to_bytes_le 32 s) in
   upd sig 63 (index sig 63 |. sign_bit)
+
 
 val verify: pk:pubkey -> plain:bytes{8 * length plain < max_size_t} -> sv:sigval -> bool
 let verify pk plain sv =
@@ -130,6 +140,7 @@ let verify pk plain sv =
   let ed_pub = upd #uint8 #32 ed_pub 31 (index #uint8 #32 ed_pub 31 |. (old_top &. u8 0x80)) in
   let sv = upd sv 63 (old_top &. u8 0x7F) in
   Spec.Ed25519.verify ed_pub plain sv
+
 
 assume type entropy
 
